theories/refinements/gradual_static/compat_cast/defs.v
@@ -1,29 +1,29 @@
-From fae_gtlc_mu.refinements.static_gradual Require Export logical_relation resources_right compat_easy help_left.
-From fae_gtlc_mu.cast_calculus Require Export types typing.
-From fae_gtlc_mu.stlc_mu Require Export lang.
+From fae_gtlc_mu.refinements.gradual_static Require Export logical_relation resources_right compat_easy.
+From fae_gtlc_mu.stlc_mu Require Export types typing.
 From fae_gtlc_mu.cast_calculus Require Export lang.
+From fae_gtlc_mu.stlc_mu Require Export lang.
 From iris.algebra Require Import list.
 From iris.proofmode Require Import tactics.
 From iris.program_logic Require Import lifting.
-From fae_gtlc_mu.cast_calculus Require Export types.
+From fae_gtlc_mu.stlc_mu Require Export types.
 From fae_gtlc_mu.cast_calculus Require Export consistency.structural.
 From fae_gtlc_mu.backtranslation Require Export cast_help.general cast_help.extract cast_help.embed.
-From fae_gtlc_mu.cast_calculus Require Export lang.
+From fae_gtlc_mu.stlc_mu Require Export lang.
 
-(* Coercion stlc_mu.lang.of_val : stlc_mu.lang.val >-> stlc_mu.lang.expr. *)
 (* Coercion cast_calculus.lang.of_val : cast_calculus.lang.val >-> cast_calculus.lang.expr. *)
+(* Coercion stlc_mu.lang.of_val : stlc_mu.lang.val >-> stlc_mu.lang.expr. *)
 
 (* Notation "# v" := (of_val v) (at level 20). *)
 
 Section defs.
   Context `{!implG Σ,!specG Σ}.
-  Notation D := (prodO stlc_mu.lang.valO cast_calculus.lang.valO -n> iPropO Σ).
-  (* Implicit Types e : stlc_mu.lang.expr. *)
-  (* Implicit Types e : stlc_mu.lang.expr. *)
+  Notation D := (prodO cast_calculus.lang.valO stlc_mu.lang.valO -n> iPropO Σ).
+  (* Implicit Types e : cast_calculus.lang.expr. *)
+  (* Implicit Types e : cast_calculus.lang.expr. *)
   Implicit Types fs : list stlc_mu.lang.val.
-  (* Implicit Types f : stlc_mu.lang.val. *)
+  (* Implicit Types f : cast_calculus.lang.val. *)
   Implicit Types A : list (cast_calculus.types.type * cast_calculus.types.type).
-  (* Implicit Types a : (cast_calculus.types.type * cast_calculus.types.type). *)
+  (* Implicit Types a : (stlc_mu.types.type * stlc_mu.types.type). *)
   Local Hint Resolve to_of_val : core.
 
   (** We will want to assume these functions to be meaningful..,
@@ -32,8 +32,9 @@ Section defs.
   Definition rel_cast_functions A (fs : list stlc_mu.lang.val) : iProp Σ :=
     ⌜length A = length fs⌝ ∗
     [∗ list] a ; f ∈ A ; fs , (
-                           □ (∀ (v : stlc_mu.lang.val) (v' : cast_calculus.lang.val) ,
-                                 ⟦ a.1 ⟧ (v , v') → ⟦ a.2 ⟧ₑ ((stlc_mu.lang.of_val f v) , Cast (v') a.1 a.2))
+                           □ (∀ (v : cast_calculus.lang.val) (v' : stlc_mu.lang.val) ,
+                                 ⟦ a.1 ⟧ (v , v') → ⟦ a.2 ⟧ₑ (Cast (v) a.1 a.2, (stlc_mu.lang.of_val f v'))
+                             )
                          )%I.
 
   Global Instance rel_cast_functions_persistent A fs :
@@ -50,6 +51,6 @@ Section defs.
   (* TODO!! 𝓕cV instead of 𝓕c *)
 
   Definition back_cast_ar {A} {τi τf} (pC : cons_struct A τi τf) :=
-  ∀ ei' K' v v' fs, (rel_cast_functions A fs ∗ ⟦ τi ⟧ (v, v') ∗ initially_inv ei' ∗ currently_half (fill K' (Cast (cast_calculus.lang.of_val v') τi τf)))
-                     ⊢ (WP (𝓕c pC fs (stlc_mu.lang.of_val v)) {{ w, ∃ w', currently_half (fill K' (cast_calculus.lang.of_val w')) ∗ ⟦ τf ⟧ (w, w') }})%I.
+    ∀ ei' K' v v' fs, (rel_cast_functions A fs ∗ ⟦ τi ⟧ (v, v') ∗ initially_inv ei' ∗ currently_half (fill K' (𝓕c pC fs (stlc_mu.lang.of_val v'))))
+                     ⊢ (WP Cast (cast_calculus.lang.of_val v) τi τf ?{{ w, ∃ w', currently_half (fill K' (stlc_mu.lang.of_val w')) ∗ ⟦ τf ⟧ (w, w') }})%I.
 End defs.
