theories/fae.v
@@ -2,8 +2,6 @@ From fae_gtlc_mu.stlc_mu Require Export contexts typing.
 From fae_gtlc_mu.cast_calculus Require Export contexts typing.
 From fae_gtlc_mu.embedding Require Export expressions types well_typedness.
 From fae_gtlc_mu.backtranslation Require Export contexts well_typedness.
-From fae_gtlc_mu.refinements.static_gradual Require Export adequacy.
-From fae_gtlc_mu.refinements.static_gradual Require Export rel_ref_specs.
 
 Notation "Γ ⊨ e '=ctx-grad=' e' : τ" :=
   (cast_calculus.contexts.ctx_equiv Γ e e' τ) (at level 74, e, e', τ at next level).
@@ -11,23 +9,39 @@ Notation "Γ ⊨ e '=ctx-grad=' e' : τ" :=
 Notation "Γ ⊨ e '=ctx-stat=' e' : τ" :=
   (stlc_mu.contexts.ctx_equiv Γ e e' τ) (at level 74, e, e', τ at next level).
 
-Lemma static_ctx_refines_gradual (Γ : list stlc_mu.types.type) (e : stlc_mu.lang.expr) (τ : stlc_mu.types.type) (de : Γ ⊢ₛ e : τ) :
-  ∀ (Cₜ : cast_calculus.contexts.ctx), cast_calculus.contexts.typed_ctx Cₜ (map embed_type Γ) (embed_type τ) [] TUnit →
-     Halts_stat (stlc_mu.contexts.fill_ctx (backtranslate_ctx Cₜ) e) →
-     Halts_grad (fill_ctx Cₜ [[e]]).
-Proof.
-  intros Cₜ dCₜ Hs.
-  apply (@adequacy actualΣ _ _ (stlc_mu.contexts.fill_ctx (backtranslate_ctx Cₜ) e) _ TUnit); auto. intros.
-  apply (back_ctx_relates (map embed_type Γ) _ _ (embed_type τ)); auto. apply (embd_closed (stlc_mu.typing.typed_closed de)).
-  by apply embedding_relates.
-Qed.
+Section static_gradual.
+  From fae_gtlc_mu.refinements.static_gradual Require Export adequacy.
+  From fae_gtlc_mu.refinements.static_gradual Require Export rel_ref_specs.
 
-Lemma gradual_ctx_refines_static (Γ : list stlc_mu.types.type) (e : stlc_mu.lang.expr) (τ : stlc_mu.types.type) :
-  ∀ (K : cast_calculus.contexts.ctx), cast_calculus.contexts.typed_ctx K (map embed_type Γ) (embed_type τ) [] TUnit →
-     Halts_grad (fill_ctx K [[e]]) →
-     Halts_stat (stlc_mu.contexts.fill_ctx (backtranslate_ctx K) e).
-Proof.
-Admitted.
+  Lemma static_ctx_refines_gradual (Γ : list stlc_mu.types.type) (e : stlc_mu.lang.expr) (τ : stlc_mu.types.type) (de : Γ ⊢ₛ e : τ) :
+    ∀ (Cₜ : cast_calculus.contexts.ctx), cast_calculus.contexts.typed_ctx Cₜ (map embed_type Γ) (embed_type τ) [] TUnit →
+       Halts_stat (stlc_mu.contexts.fill_ctx (backtranslate_ctx Cₜ) e) →
+       Halts_grad (fill_ctx Cₜ [[e]]).
+  Proof.
+    intros Cₜ dCₜ Hs.
+    apply (@adequacy actualΣ _ _ (stlc_mu.contexts.fill_ctx (backtranslate_ctx Cₜ) e) _ TUnit); auto. intros.
+    apply (back_ctx_relates (map embed_type Γ) _ _ (embed_type τ)); auto. apply (embd_closed (stlc_mu.typing.typed_closed de)).
+    by apply embedding_relates.
+  Qed.
+
+End static_gradual.
+
+Section gradual_static.
+  From fae_gtlc_mu.refinements.gradual_static Require Export adequacy.
+  From fae_gtlc_mu.refinements.gradual_static Require Export rel_ref_specs.
+
+  Lemma gradual_ctx_refines_static (Γ : list stlc_mu.types.type) (e : stlc_mu.lang.expr) (τ : stlc_mu.types.type) (de : Γ ⊢ₛ e : τ ):
+    ∀ (K : cast_calculus.contexts.ctx), cast_calculus.contexts.typed_ctx K (map embed_type Γ) (embed_type τ) [] TUnit →
+       Halts_grad (fill_ctx K [[e]]) →
+       Halts_stat (stlc_mu.contexts.fill_ctx (backtranslate_ctx K) e).
+  Proof.
+    intros Cₜ dCₜ Hs.
+    apply (@adequacy actualΣ _ _ (fill_ctx Cₜ [[e]]) (stlc_mu.contexts.fill_ctx (backtranslate_ctx Cₜ) e) TUnit); auto. intros.
+    apply (back_ctx_relates (map embed_type Γ) _ _ (embed_type τ)); auto. apply (embd_closed (stlc_mu.typing.typed_closed de)).
+    by apply embedding_relates.
+  Qed.
+
+End gradual_static.
 
 Definition retract τ : backtranslate_type (embed_type τ) = τ.
 Proof. induction τ; simpl; try done; try by rewrite IHτ1 IHτ2. by rewrite IHτ. Qed.
@@ -47,7 +61,7 @@ Proof.
            (map backtranslate_type []) (backtranslate_type $ embed_type stlc_mu.types.TUnit)).
     repeat rewrite retract. rewrite map_map (map_ext _ id _ (Γ)). by rewrite (map_id Γ). intro; by rewrite retract.
     apply well_typedness_ctx. apply (embd_closed (stlc_mu.typing.typed_closed pe1)). auto.
-    by apply (gradual_ctx_refines_static Γ e1 τ Cₜ dCₜ).
+    by apply (gradual_ctx_refines_static Γ e1 τ pe1 Cₜ dCₜ).
   - intro Hg2.
     apply (static_ctx_refines_gradual Γ e1 τ (ltac:(apply Hctx)) Cₜ dCₜ).
     apply Hctx.
@@ -57,6 +71,6 @@ Proof.
            (map backtranslate_type []) (backtranslate_type $ embed_type stlc_mu.types.TUnit)).
     repeat rewrite retract. rewrite map_map (map_ext _ id _ (Γ)). by rewrite (map_id Γ). intro; by rewrite retract.
     apply well_typedness_ctx. apply (embd_closed (stlc_mu.typing.typed_closed pe1)). auto.
-    apply (gradual_ctx_refines_static Γ e2 τ Cₜ dCₜ).
+    apply (gradual_ctx_refines_static Γ e2 τ pe2 Cₜ dCₜ).
     apply Hg2.
 Qed.
