theories/refinements/gradual_static/adequacy.v
@@ -1,0 +1,61 @@
+From iris.algebra Require Import excl auth frac agree.
+From iris.proofmode Require Import tactics.
+From iris.program_logic Require Import adequacy.
+From iris.algebra Require Import agree.
+
+From fae_gtlc_mu Require Import cast_calculus.lang stlc_mu.lang.
+From fae_gtlc_mu Require Import refinements.gradual_static.logical_relation.
+From fae_gtlc_mu Require Import refinements.gradual_static.compat_easy. (* just for notation *)
+
+Definition Halts_grad := cast_calculus.lang.Halts.
+
+Definition Halts_stat := stlc_mu.lang.Halts.
+
+Section adequacy.
+  Context `{!inG Σ specR, !invPreG Σ}.
+
+  Lemma adequacy
+    (e : cast_calculus.lang.expr) (e' : stlc_mu.lang.expr) (τ : cast_calculus.types.type) :
+    (∀ `{!implG Σ, !specG Σ}, [] ⊨ e ≤log≤ e' : τ) →
+    (Halts_grad e) →
+    (Halts_stat e').
+  Proof.
+    intros Hlog Hsteps.
+    cut (adequate MaybeStuck e tt (λ _ _, ∃ v', rtc erased_step ([e'], tt) (of_val v' :: [], tt))).
+    { rewrite /Halts_grad in Hsteps. rewrite /cast_calculus.lang.Halts in Hsteps. destruct 1. naive_solver. }
+    eapply (wp_adequacy Σ); first by apply _.
+    iIntros (Hinv ?).
+    iMod (own_alloc ((((1/2)%Qp , to_agree e') ⋅ ((1/2)%Qp , to_agree e')) : specR)) as (spec_name) "[Hs1 Hs2]".
+    { rewrite -pair_op frac_op' Qp_half_half agree_idemp.
+      apply pair_valid; split; try done; try by apply frac_valid'. }
+    set (SpecΣ := SpecG Σ inG0 spec_name).
+    set (ImplΣ := ImplG Σ Hinv).
+    iMod (inv_alloc specN _ (initially_body e') with "[Hs1]") as "#Hinitially".
+    { iNext. iExists e'. iSplit; eauto. }
+    iExists (λ _ _, True%I), (λ _, True%I); iSplitR; first done.
+    iApply wp_fupd. iApply (wp_wand with "[-]").
+    - iPoseProof (Hlog ImplΣ SpecΣ [] e' with "[]") as "Hrel".
+      { iSplit; auto. iApply interp_env_nil. }
+      replace e with (e.[cast_calculus.typing.env_subst [] ]) at 2 by by asimpl.
+      iApply ("Hrel" $! []). asimpl; iFrame.
+    - iModIntro. simpl. iIntros (v'). iDestruct 1 as (v2) "[Hj #Hinterp]".
+      iExists v2.
+      iInv specN as ">Hinv" "Hclose".
+      iDestruct "Hinv" as (e'') "[He'' %]".
+      iDestruct (own_valid_2 with "He'' Hj") as %Hvalid.
+      rewrite -pair_op frac_op' Qp_half_half in Hvalid.
+      move: Hvalid=> /pair_valid [_ /agree_op_inv' b]. apply leibniz_equiv in b. subst.
+      iMod ("Hclose" with "[-]") as "_".
+      + iExists (#v2). auto.
+      + iIntros "!> !%". eauto.
+  Qed.
+
+End adequacy.
+
+Definition actualΣ : gFunctors := #[ invΣ ; GFunctor specR ].
+
+Instance subG_inG_specR {Σ} : subG (GFunctor specR) Σ → inG Σ specR.
+Proof. solve_inG. Qed.
+
+(* Lemma actualΣ_inG_specR : invPreG actualΣ. *)
+(* Proof. apply subG_invΣ. rewrite /actualΣ. solve_inG. :( *)
