theories/refinements/gradual_static/compat_cast/all.v
@@ -1,28 +1,22 @@
-From fae_gtlc_mu.refinements.static_gradual Require Export logical_relation resources_right compat_easy help_left compat_cast.defs.
-From fae_gtlc_mu.cast_calculus Require Export types typing.
-From fae_gtlc_mu.stlc_mu Require Export lang.
+From fae_gtlc_mu.stlc_mu Require Export types typing.
 From fae_gtlc_mu.cast_calculus Require Export lang.
 From iris.algebra Require Import list.
 From iris.proofmode Require Import tactics.
 From iris.program_logic Require Import lifting.
-From fae_gtlc_mu.cast_calculus Require Export types.
-From fae_gtlc_mu.cast_calculus Require Export consistency.structural.
 From fae_gtlc_mu.backtranslation Require Export cast_help.general cast_help.extract cast_help.embed.
-From fae_gtlc_mu.refinements.static_gradual.compat_cast Require Export between_rec prod_prod sum_sum arrow_arrow identity tau_star ground_star tau_star star_tau star_ground.
+From fae_gtlc_mu.stlc_mu Require Export lang.
+From fae_gtlc_mu.refinements.gradual_static Require Export logical_relation resources_left resources_right compat_easy compat_cast.defs.
+From fae_gtlc_mu.cast_calculus Require Export consistency.structural types.
+From fae_gtlc_mu.refinements.gradual_static.compat_cast Require Export between_rec prod_prod sum_sum arrow_arrow identity tau_star ground_star tau_star star_tau star_ground.
 
 Section compat_cast_all.
   Context `{!implG Σ,!specG Σ}.
-  Notation D := (prodO stlc_mu.lang.valO cast_calculus.lang.valO -n> iPropO Σ).
-  (* Implicit Types e : stlc_mu.lang.expr. *)
-  (* Implicit Types e : stlc_mu.lang.expr. *)
+  Notation D := (prodO cast_calculus.lang.valO stlc_mu.lang.valO -n> iPropO Σ).
   Implicit Types fs : list stlc_mu.lang.val.
   (* Implicit Types f : stlc_mu.lang.val. *)
   Implicit Types A : list (cast_calculus.types.type * cast_calculus.types.type).
-  (* Implicit Types a : (cast_calculus.types.type * cast_calculus.types.type). *)
   Local Hint Resolve to_of_val : core.
-  Local Hint Resolve stlc_mu.lang.to_of_val : core.
-
-  (** Proving it *)
+  Local Hint Resolve cast_calculus.lang.to_of_val : core.
 
   Lemma back_cast_ar_all {A} {τi τf} (pC : cons_struct A τi τf) : back_cast_ar pC.
   Proof.
@@ -40,24 +34,22 @@ Section compat_cast_all.
     - by apply back_cast_ar_trec_trec_use.
   Qed.
 
-
   Notation "'` H" := (bin_log_related_alt H) (at level 8).
 
   Lemma bin_log_related_back_cast Γ e e' τi τf (pC : cons_struct [] τi τf)
       (IHHtyped : Γ ⊨ e ≤log≤ e' : τi) :
-    Γ ⊨ 𝓕c pC [] e ≤log≤ Cast e' τi τf : τf.
+    Γ ⊨ Cast e τi τf ≤log≤ 𝓕c pC [] e' : τf.
   Proof.
     iIntros (vvs ei) "#[Hρ HΓ]"; iIntros (K) "Hj /=".
     rewrite 𝓕c_closed; try auto.
     rewrite 𝓕c_rewrite.
-    iApply (wp_bind (ectx_language.fill [stlc_mu.lang.AppRCtx _])).
-    iApply (wp_wand with "[Hj]"). iApply ('`IHHtyped _ _ (CastCtx τi τf :: K)). iFrame. auto.
+    iApply (wp_bind [CastCtx _ _]). iApply (wp_wand with "[-]").
+    iApply ('`IHHtyped _ _ (AppRCtx _ :: K)). auto.
     iIntros (v). iDestruct 1 as (v') "[Hv' Hvv']". simpl.
     rewrite -𝓕c_rewrite.
     iApply (wp_wand with "[-]").
     iApply ((back_cast_ar_all pC) with "[-]").
-    iSplitR. unfold rel_cast_functions. iSplit; auto.
-    iSplitL "Hvv'". auto. auto.
+    iSplitR; auto. unfold rel_cast_functions. by iSplit; auto.
     clear v v'.
     iIntros (v). iDestruct 1 as (v') "[Hv' Hvv']".
     iExists v'.
@@ -65,10 +57,10 @@ Section compat_cast_all.
   Qed.
 
   Lemma bin_log_related_omega Γ e' τ :
-    Γ ⊨ Ω ≤log≤ e' : τ.
+    Γ ⊨ CastError ≤log≤ e' : τ.
   Proof.
     iIntros (vvs ρ) "#[Hρ HΓ]"; iIntros (K) "Hj /=".
-    by iApply wp_Ω.
+    by iApply wp_CastError'.
   Qed.
 
 End compat_cast_all.
