theories/refinements/gradual_static/compat_cast/between_rec.v
@@ -1,22 +1,24 @@
-From fae_gtlc_mu.refinements.static_gradual Require Export logical_relation resources_right compat_easy help_left compat_cast.defs.
-From fae_gtlc_mu.cast_calculus Require Export types typing.
+From fae_gtlc_mu.stlc_mu Require Export types typing.
 From fae_gtlc_mu.cast_calculus Require Export lang.
 From iris.algebra Require Import list.
 From iris.proofmode Require Import tactics.
 From iris.program_logic Require Import lifting.
-From fae_gtlc_mu.cast_calculus Require Export consistency.structural.
 From fae_gtlc_mu.backtranslation Require Export cast_help.general cast_help.extract cast_help.embed cast_help.props.between_rec_fix.
-From fae_gtlc_mu.cast_calculus Require Export lang types.
+From fae_gtlc_mu.stlc_mu Require Export lang.
+From fae_gtlc_mu.refinements.gradual_static Require Export logical_relation resources_left resources_right compat_easy compat_cast.defs.
+From fae_gtlc_mu.cast_calculus Require Export consistency.structural types.
 
 Section between_rec.
   Context `{!implG Σ,!specG Σ}.
-  Notation D := (prodO stlc_mu.lang.valO cast_calculus.lang.valO -n> iPropO Σ).
-  (* Implicit Types e : stlc_mu.lang.expr. *)
+  Notation D := (prodO cast_calculus.lang.valO stlc_mu.lang.valO -n> iPropO Σ).
+  (* Implicit Types e : cast_calculus.lang.expr. *)
   Implicit Types fs : list stlc_mu.lang.val.
-  (* Implicit Types f : stlc_mu.lang.val. *)
+  (* Implicit Types f : cast_calculus.lang.val. *)
   Implicit Types A : list (cast_calculus.types.type * cast_calculus.types.type).
-  (* Implicit Types a : (cast_calculus.types.type * cast_calculus.types.type). *)
+  (* Implicit Types a : (stlc_mu.types.type * stlc_mu.types.type). *)
   Local Hint Resolve to_of_val : core.
+
+  Hint Extern 5 (AsVal _) => eexists; simpl; try done; eapply cast_calculus.lang.of_to_val; fast_done : typeclass_instances.
 
   (** Proving it *)
 
@@ -48,46 +50,33 @@ Section between_rec.
   Proof.
     intros A τl τr pμτlμτrnotA pC IHpC.
     rewrite /𝓕c /𝓕 /back_cast_ar; iIntros (ei' K' v v' fs) "(#Hfs & #Hvv' & #Hei' & Hv')".
+    iDestruct "Hfs" as "[% Hfs']"; iAssert (rel_cast_functions A fs) with "[Hfs']" as "Hfs". iSplit; done. rename H into Hl.
     (** setting up iLöb *)
     iLöb as "IHlob" forall (v v' ei' K') "Hvv' Hei'".
-    (* fold (𝓕c (consTRecTRecExposeCall A τl τr pμτlμτrnotA pC) fs). *)
-    (* iRevert (ei' K' v v') "Hvv' Hei' Hv'". *)
+    (** ... *)
     rewrite {2}/𝓕c. rewrite /𝓕.
     fold (𝓕 pC).
     (** rewriting value relation for v and v' *)
-    (* rewrite fixpoint_interp_rec1_eq. *)
     rewrite interp_rw_TRec.
     iDestruct "Hvv'" as (w w') "#[% Hww']".
     inversion H; clear v v' H H1 H2.
-    (** evaluation steps in WP *)
-    iDestruct "Hfs" as "[% Hfs']"; iAssert (rel_cast_functions A fs) with "[Hfs']" as "Hfs". iSplit; done.
-    iApply (wp_pure_step_later _ _ _ (stlc_mu.lang.Fold ((𝓕c pC (𝓕cV (consTRecTRecExposeCall A τl τr pμτlμτrnotA pC) fs H :: fs)) w)) True); auto. intros _. apply between_TRec_steps.
-    (** WP *)
-    repeat iModIntro.
-    iApply (wp_bind (stlc_mu.lang.fill_item $ stlc_mu.lang.FoldCtx)).
-    (** eval specification side *)
-    iMod (step_pure _ ei' K'
-                    (Cast (Fold w') (TRec τl) (TRec τr))
-                    (Fold (Cast (Unfold (Fold w')) (τl.[TRec τl/]) (τr.[TRec τr/]))) with "[Hv']") as "Hv'".
-    intros. apply (RecursiveCast _ (FoldV w')). by rewrite -to_of_val. auto. by iFrame.
-    iMod (step_pure _ ei' (CastCtx τl.[TRec τl/] τr.[TRec τr/] :: FoldCtx :: K')
-                    (Unfold (Fold (# w')))
-                    w' with "[Hv']") as "Hv'".
-    intros. apply (Unfold_Fold _ w'). by rewrite to_of_val. auto. by iFrame.
-    (** apply IH *)
-
+    (** implementation side *)
+    wp_head.
+    iApply (wp_bind [CastCtx _ _; cast_calculus.lang.FoldCtx]).
+    wp_head. fold (cast_calculus.lang.of_val w). wp_value. simpl (lang.fill _ _).
+    (** specification side *)
+    iMod (steps_pure _ ei' K' _ _ _ (between_TRec_steps pC fs Hl pμτlμτrnotA w') with "[Hv']") as "Hv'"; auto.
+    (** IH *)
+    iApply (wp_bind [cast_calculus.lang.FoldCtx]).
     iApply (wp_wand with "[-]").
-    iApply (IHpC ei' (FoldCtx :: K') w w' (𝓕cV (consTRecTRecExposeCall A τl τr pμτlμτrnotA pC) fs H :: fs)). iSplitL "Hfs". iSplitR. simpl. by rewrite H.
-    (** applying IHlob and Hfs *)
-    (* rewrite /𝓕c. *)
-    iSplit.
+    iApply (IHpC ei' (FoldCtx :: K') w w' (𝓕cV (consTRecTRecExposeCall A τl τr pμτlμτrnotA pC) fs Hl :: fs)).
+    iFrame "Hei' Hww' Hv'". iSplit; first by (simpl; iPureIntro; lia). iSplit; try done.
+    (** iLob *)
     iModIntro. iIntros (v v') "#Hvv'".
-    { clear K'. iIntros (K') "Hv'". iSimpl in "Hv'".
-      rewrite -𝓕c_rewrite.
-      iApply ("IHlob" $! v v' with "Hv' Hvv' Hei'").
-    }
-    done. iSplitR. done. iSplitR. done. by simpl.
-    (** finish *)
+    clear K'. iIntros (K') "Hv'". iSimpl in "Hv'".
+    rewrite -𝓕c_rewrite.
+    iApply ("IHlob" $! v v' with "Hv' Hvv' Hei'").
+    (** ... *)
     iIntros (v) "H".
     iDestruct "H" as (v') "[Hv' #Hvv']".
     iApply wp_value.
@@ -95,8 +84,7 @@ Section between_rec.
     iFrame.
     rewrite interp_rw_TRec.
     simpl. iModIntro.
-    iExists v , v'.
-    iSplitR. done. auto.
+    iExists v , v'; auto.
   Qed.
 
 End between_rec.
