theories/refinements/gradual_static/compat_cast/identity.v
@@ -1,0 +1,45 @@
+From fae_gtlc_mu.stlc_mu Require Export types typing.
+From fae_gtlc_mu.cast_calculus Require Export lang.
+From iris.algebra Require Import list.
+From iris.proofmode Require Import tactics.
+From iris.program_logic Require Import lifting.
+From fae_gtlc_mu.backtranslation Require Export cast_help.general cast_help.extract cast_help.embed.
+From fae_gtlc_mu.stlc_mu Require Export lang.
+From fae_gtlc_mu.refinements.gradual_static Require Export logical_relation resources_left resources_right compat_easy compat_cast.defs.
+From fae_gtlc_mu.cast_calculus Require Export consistency.structural types.
+
+Section compat_cast_identity.
+  Context `{!implG Σ,!specG Σ}.
+  Notation D := (prodO cast_calculus.lang.valO stlc_mu.lang.valO -n> iPropO Σ).
+  (* Implicit Types e : cast_calculus.lang.expr. *)
+  (* Implicit Types e : cast_calculus.lang.expr. *)
+  Implicit Types fs : list cast_calculus.lang.val.
+  (* Implicit Types f : cast_calculus.lang.val. *)
+  (* Implicit Types a : (stlc_mu.types.type * stlc_mu.types.type). *)
+  Local Hint Resolve to_of_val : core.
+  Local Hint Resolve cast_calculus.lang.to_of_val : core.
+
+
+  Hint Extern 5 (AsVal _) => eexists; simpl; try done; eapply cast_calculus.lang.of_to_val; fast_done : typeclass_instances.
+
+  Lemma back_cast_ar_base_base:
+    ∀ A : list (type * type), back_cast_ar (consBaseBase A).
+  Proof.
+    intros A.
+    rewrite /back_cast_ar. iIntros (ei' K' v v' fs) "(#Hfs & #Hvv' & #Hei' & Hv')".
+    rewrite /𝓕c /𝓕. asimpl.
+    iMod ((step_lam _ ei' K') with "[Hv']") as "Hv'"; auto; simpl.
+    wp_head. wp_value. iExists v'. auto.
+  Qed.
+
+  Lemma back_cast_ar_star_star:
+    ∀ A : list (type * type), back_cast_ar (consStarStar A).
+  Proof.
+    intros A.
+    rewrite /back_cast_ar. iIntros (ei' K' v v' fs) "(#Hfs & #Hvv' & #Hei' & Hv')".
+    rewrite /𝓕c /𝓕. asimpl.
+    iMod ((step_lam _ ei' K') with "[Hv']") as "Hv'"; auto; simpl.
+    wp_head. wp_value. iExists v'. auto.
+  Qed.
+
+End compat_cast_identity.
