theories/refinements/gradual_static/compat_cast/prod_prod.v
@@ -1,0 +1,73 @@
+From fae_gtlc_mu.stlc_mu Require Export types typing.
+From fae_gtlc_mu.cast_calculus Require Export lang.
+From iris.algebra Require Import list.
+From iris.proofmode Require Import tactics.
+From iris.program_logic Require Import lifting.
+From fae_gtlc_mu.backtranslation Require Export cast_help.general cast_help.extract cast_help.embed.
+From fae_gtlc_mu.stlc_mu Require Export lang.
+From fae_gtlc_mu.refinements.gradual_static Require Export logical_relation resources_left resources_right compat_easy compat_cast.defs.
+From fae_gtlc_mu.cast_calculus Require Export consistency.structural types.
+
+Section compat_cast_prod_prod.
+  Context `{!implG Σ,!specG Σ}.
+  Notation D := (prodO cast_calculus.lang.valO stlc_mu.lang.valO -n> iPropO Σ).
+  (* Implicit Types e : cast_calculus.lang.expr. *)
+  (* Implicit Types e : cast_calculus.lang.expr. *)
+  Implicit Types fs : list cast_calculus.lang.val.
+  (* Implicit Types f : cast_calculus.lang.val. *)
+  Implicit Types A : list (stlc_mu.types.type * stlc_mu.types.type).
+  (* Implicit Types a : (stlc_mu.types.type * stlc_mu.types.type). *)
+  Local Hint Resolve to_of_val : core.
+  Local Hint Resolve cast_calculus.lang.to_of_val : core.
+
+
+  Hint Resolve to_of_val : core.
+
+  Hint Extern 5 (AsVal _) => eexists; simpl; try done; eapply cast_calculus.lang.of_to_val; fast_done : typeclass_instances.
+  Hint Extern 10 (AsVal _) =>
+  eexists; rewrite /IntoVal; eapply of_to_val; rewrite /= !to_of_val /=; solve [ eauto ] : typeclass_instances.
+
+  Lemma back_cast_ar_prod_prod:
+    ∀ (A : list (type * type)) (τ1 τ1' τ2 τ2' : type) (pC1 : cons_struct A τ1 τ1') (pC2 : cons_struct A τ2 τ2')
+      (IHpC1 : back_cast_ar pC1) (IHpC2 : back_cast_ar pC2),
+      back_cast_ar (consTProdTProd A τ1 τ1' τ2 τ2' pC1 pC2).
+  Proof.
+    intros A τ1 τ1' τ2 τ2' pC1 pC2 IHpC1 IHpC2.
+    rewrite /back_cast_ar. iIntros (ei' K' v v' fs) "(#Hfs & #Hvv' & #Hei' & Hv')".
+    iDestruct "Hfs" as "[% Hfs']"; iAssert (rel_cast_functions A fs) with "[Hfs']" as "Hfs". iSplit; done. iClear "Hfs'".
+    rewrite /𝓕c /𝓕. fold (𝓕 pC1) (𝓕 pC2). rewrite between_TProd_subst_rewrite. fold (𝓕c pC1 fs) (𝓕c pC2 fs).
+    rewrite interp_rw_TProd.
+    iDestruct "Hvv'" as ((v1, v1') (v2, v2')) "(% & #H1 & #H2)". simpl in H0. inversion H0. clear H0 H2 H3 v v'.
+    (** impl side *)
+    wp_head.
+    iApply (wp_bind [CastCtx _ _ ; cast_calculus.lang.PairLCtx _]). wp_head. wp_value. simpl.
+    (** spec side *)
+    rewrite /between_TProd.
+    assert (Pair (of_val v1') (of_val v2') = of_val (PairV v1' v2')) as ->. by simpl.
+    iMod ((step_lam _ ei' K') with "[Hv']") as "Hv'"; auto. asimpl.
+    rewrite 𝓕c_rewrite.
+    iMod ((step_fst _ ei' (AppRCtx _ :: PairLCtx _ :: K')) with "[Hv']") as "Hv'"; auto. simpl.
+    rewrite -𝓕c_rewrite.
+    (** first IH *)
+    iApply (wp_bind [cast_calculus.lang.PairLCtx _ ]). iApply (wp_wand with "[-]").
+    iApply (IHpC1 ei' (PairLCtx _ :: K') with "[Hv' Hfs]"). auto.
+    (** .... *)
+    iIntros (v1f) "HHH". iDestruct "HHH" as (v1f') "[Hv2' #Hv1fv1f']". simpl.
+    (** impl side *)
+    iApply (wp_bind [CastCtx _ _ ; cast_calculus.lang.PairRCtx _]). wp_head. wp_value. simpl.
+    (** spec side *)
+    rewrite 𝓕c_rewrite.
+    iMod ((step_snd _ ei' (AppRCtx _ :: PairRCtx _ :: K')) with "[Hv2']") as "Hv2'"; auto. simpl.
+    rewrite -𝓕c_rewrite.
+    (** second IH *)
+    iApply (wp_bind [cast_calculus.lang.PairRCtx _]). iApply (wp_wand with "[-]").
+    iApply (IHpC2 ei' (PairRCtx _ :: K') with "[Hv2' Hfs]"). auto.
+    (** .... *)
+    iIntros (v2f) "HHH". iDestruct "HHH" as (v2f') "[Hvf #Hv2fv2f']". simpl.
+    wp_value.
+    iExists (PairV v1f' v2f'). iSplitL. done.
+    rewrite interp_rw_TProd.
+    iExists (v1f , v1f') , (v2f , v2f') . auto.
+Qed.
+
+End compat_cast_prod_prod.
