theories/refinements/gradual_static/compat_cast/tau_star.v
@@ -1,0 +1,54 @@
+From fae_gtlc_mu.stlc_mu Require Export types typing.
+From fae_gtlc_mu.cast_calculus Require Export lang.
+From iris.algebra Require Import list.
+From iris.proofmode Require Import tactics.
+From iris.program_logic Require Import lifting.
+From fae_gtlc_mu.backtranslation Require Export cast_help.general.
+From fae_gtlc_mu.stlc_mu Require Export lang.
+From fae_gtlc_mu.refinements.gradual_static Require Export logical_relation resources_left resources_right compat_easy compat_cast.defs.
+From fae_gtlc_mu.cast_calculus Require Export consistency.structural types.
+
+
+Section compat_cast_tau_star.
+  Context `{!implG Σ,!specG Σ}.
+  Notation D := (prodO cast_calculus.lang.valO stlc_mu.lang.valO -n> iPropO Σ).
+  (* Implicit Types e : cast_calculus.lang.expr. *)
+  (* Implicit Types e : cast_calculus.lang.expr. *)
+  Implicit Types fs : list cast_calculus.lang.val.
+  (* Implicit Types f : cast_calculus.lang.val. *)
+  Implicit Types A : list (stlc_mu.types.type * stlc_mu.types.type).
+  (* Implicit Types a : (stlc_mu.types.type * stlc_mu.types.type). *)
+  Local Hint Resolve to_of_val : core.
+  Local Hint Resolve cast_calculus.lang.to_of_val : core.
+
+  (** Proving it *)
+
+  Hint Extern 5 (AsVal _) => eexists; simpl; try done; eapply cast_calculus.lang.of_to_val; fast_done : typeclass_instances.
+
+  Lemma back_cast_ar_tau_star:
+    ∀ (A : list (type * type)) (τ τG : type) (pτnG : Ground τ → False) (pτnStar : τ ≠ ⋆) (pτSτG : get_shape τ = Some τG) (pC1 : cons_struct A τ τG) (pC2 : cons_struct A τG ⋆),
+      back_cast_ar pC1 → back_cast_ar pC2 → back_cast_ar (consTauStar A τ τG pτnG pτnStar pτSτG pC1 pC2).
+  Proof.
+    intros A τ τG pτnG pτnStar pτSτG pC1 pC2 IHpC1 IHpC2.
+    iIntros (ei' K' v v' fs) "(#Hfs & #Hvv' & #Hei' & Hv')".
+    rewrite /back_cast_ar /𝓕c /𝓕. rewrite factorization_subst_rewrite. fold (𝓕 pC1). fold (𝓕 pC2).
+    fold (𝓕c pC1 fs). fold (𝓕c pC2 fs). rewrite /factorization.
+    iDestruct "Hfs" as "[% Hfs']"; iAssert (rel_cast_functions A fs) with "[Hfs']" as "Hfs". iSplit; done. iClear "Hfs'".
+    (** implementation *)
+    iApply wp_pure_step_later; try auto. apply pure_fact_up; auto. done. by eauto; eexists. simpl. done. iNext.
+    (** specification *)
+    iMod ((step_lam _ ei' K') with "[Hv']") as "Hv'"; auto. asimpl.
+    (** first IH *)
+    rewrite 𝓕c_rewrite.
+    iApply (wp_bind [CastCtx _ _]). iApply (wp_wand with "[-]").
+    iApply (IHpC1 ei' (AppRCtx _ :: K') with "[Hv']"); auto.
+    (** .... *)
+    iIntros (w) "blaa".  iDestruct "blaa" as (w') "[Hw' #Hww']".
+    simpl. rewrite -𝓕c_rewrite.
+    (** second IH *)
+    iApply (wp_wand with "[-]").
+    iApply (IHpC2 ei' K' with "[Hw']"); auto.
+    auto.
+  Qed.
+
+End compat_cast_tau_star.
