theories/refinements/gradual_static/compat_easy.v
@@ -1,33 +1,34 @@
-From fae_gtlc_mu.refinements.static_gradual Require Export resources_right logical_relation.
-From fae_gtlc_mu.cast_calculus Require Export types typing.
+From fae_gtlc_mu.stlc_mu Require Export types typing.
+From fae_gtlc_mu.cast_calculus Require Export lang.
 From fae_gtlc_mu.stlc_mu Require Export lang.
-From fae_gtlc_mu.cast_calculus Require Export lang.
-From fae_gtlc_mu.cast_calculus Require Export lang.
+From fae_gtlc_mu.stlc_mu Require Export lang.
 From iris.algebra Require Import list.
 From iris.proofmode Require Import tactics.
 From iris.program_logic Require Import lifting.
+From fae_gtlc_mu.refinements.gradual_static Require Export resources_right logical_relation.
+From fae_gtlc_mu.stlc_mu Require Export lang.
 
 Notation "Γ ⊨ e '≤log≤' e' : τ" :=
   (bin_log_related Γ e e' τ) (at level 74, e, e', τ at next level).
 
 Section fundamental.
   Context `{!implG Σ,!specG Σ}.
-  Notation D := (prodO stlc_mu.lang.valO cast_calculus.lang.valO -n> iPropO Σ).
-  (* Implicit Types e : stlc_mu.lang.expr. *)
+  Notation D := (prodO cast_calculus.lang.valO stlc_mu.lang.valO -n> iPropO Σ).
+  (* Implicit Types e : cast_calculus.lang.expr. *)
   Local Hint Resolve to_of_val : core.
 
   Local Tactic Notation "smart_wp_bind" uconstr(ctx) ident(v) ident(w)
         constr(Hv) uconstr(Hp) :=
-    iApply (wp_bind (ectx_language.fill [ctx]));
+    iApply (wp_bind ([ctx]));
     iApply (wp_wand with "[-]");
       [iApply Hp; iFrame "#"; trivial|];
     iIntros (v); iDestruct 1 as (w) Hv.
 
   (* Put all quantifiers at the outer level *)
   Lemma bin_log_related_alt {Γ e e' τ} : Γ ⊨ e ≤log≤ e' : τ → ∀ vvs ei' K',
-    initially_inv ei' ∗ ⟦ Γ ⟧* vvs ∗ currently_half (fill K' (e'.[cast_calculus.typing.env_subst (vvs.*2)]))
-    ⊢ WP e.[stlc_mu.typing.env_subst (vvs.*1)] {{ v, ∃ v',
-        currently_half (fill K' (cast_calculus.lang.of_val v')) ∗ interp τ (v, v') }}.
+    initially_inv ei' ∗ ⟦ Γ ⟧* vvs ∗ currently_half (ectx_language.fill K' (e'.[stlc_mu.typing.env_subst (vvs.*2)]))
+    ⊢ WP e.[cast_calculus.typing.env_subst (vvs.*1)] ?{{ v, ∃ v',
+        currently_half (ectx_language.fill K' (stlc_mu.lang.of_val v')) ∗ interp τ (v, v') }}.
   Proof.
     iIntros (Hlog vvs K ρ) "[#Hρ [HΓ Hj]]". asimpl.
     iApply (Hlog with "[HΓ]"); iFrame. eauto.
@@ -36,33 +37,33 @@ Section fundamental.
   Notation "'` H" := (bin_log_related_alt H) (at level 8).
 
   Lemma bin_log_related_var Γ x τ :
-    Γ !! x = Some τ → Γ ⊨ stlc_mu.lang.Var x ≤log≤ cast_calculus.lang.Var x : τ.
+    Γ !! x = Some τ → Γ ⊨ cast_calculus.lang.Var x ≤log≤ stlc_mu.lang.Var x : τ.
   Proof.
     iIntros (? vvs ei') "[#Hρ #HΓ]". iIntros (K). iIntros "Hj /=".
     iDestruct (interp_env_Some_l with "HΓ") as ([v v']) "[Heq Hv]"; first done.
     iDestruct "Heq" as %Heq.
-    erewrite !stlc_mu.typing.env_subst_lookup; rewrite ?list_lookup_fmap ?Heq; eauto.
     erewrite !cast_calculus.typing.env_subst_lookup; rewrite ?list_lookup_fmap ?Heq; eauto.
+    erewrite !stlc_mu.typing.env_subst_lookup; rewrite ?list_lookup_fmap ?Heq; eauto.
     iApply wp_value. eauto.
   Qed.
 
-  Lemma bin_log_related_unit Γ : Γ ⊨ stlc_mu.lang.Unit ≤log≤ cast_calculus.lang.Unit : TUnit.
+  Lemma bin_log_related_unit Γ : Γ ⊨ cast_calculus.lang.Unit ≤log≤ stlc_mu.lang.Unit : TUnit.
   Proof.
     iIntros (vvs ei') "#[Hρ HΓ]". iIntros (K) "Hj /=".
-    iApply wp_value. iExists UnitV. rewrite unfold_interp_type_pair. eauto.
+    iApply wp_value. iExists stlc_mu.lang.UnitV. rewrite unfold_interp_type_pair. eauto.
   Qed.
 
   Lemma bin_log_related_pair Γ e1 e2 e1' e2' τ1 τ2
       (IHHtyped1 : Γ ⊨ e1 ≤log≤ e1' : τ1)
       (IHHtyped2 : Γ ⊨ e2 ≤log≤ e2' : τ2) :
-    Γ ⊨ stlc_mu.lang.Pair e1 e2 ≤log≤ Pair e1' e2' : TProd τ1 τ2.
+    Γ ⊨ cast_calculus.lang.Pair e1 e2 ≤log≤ stlc_mu.lang.Pair e1' e2' : TProd τ1 τ2.
   Proof.
     iIntros (vvs ei') "#[Hρ HΓ]"; iIntros (K) "Hj /=".
-    smart_wp_bind (stlc_mu.lang.PairLCtx e2.[stlc_mu.typing.env_subst _]) v v' "[Hv #Hiv]"
-      ('`IHHtyped1 _ _ ((cast_calculus.lang.PairLCtx e2'.[env_subst _]) :: K)).
+    smart_wp_bind (cast_calculus.lang.PairLCtx e2.[cast_calculus.typing.env_subst _]) v v' "[Hv #Hiv]"
+      ('`IHHtyped1 _ _ ((stlc_mu.lang.PairLCtx e2'.[stlc_mu.typing.env_subst _]) :: K)).
       (* ('`IHHtyped1 _ _ ((PairLCtx e2'.[env_subst _]) :: K)). *)
-    smart_wp_bind (stlc_mu.lang.PairRCtx v) w w' "[Hw #Hiw]"
-      ('`IHHtyped2 _ _ ((PairRCtx v') :: K)).
+    smart_wp_bind (cast_calculus.lang.PairRCtx v) w w' "[Hw #Hiw]"
+      ('`IHHtyped2 _ _ ((stlc_mu.lang.PairRCtx v') :: K)).
     iApply wp_value.
     iExists (PairV v' w'); iFrame "Hw".
     rewrite interp_rw_TProd.
@@ -71,10 +72,10 @@ Section fundamental.
 
   Lemma bin_log_related_fst Γ e e' τ1 τ2
       (IHHtyped : Γ ⊨ e ≤log≤ e' : TProd τ1 τ2) :
-    Γ ⊨ stlc_mu.lang.Fst e ≤log≤ Fst e' : τ1.
+    Γ ⊨ cast_calculus.lang.Fst e ≤log≤ Fst e' : τ1.
   Proof.
     iIntros (vvs ei') "[#Hρ #HΓ]"; iIntros (K) "Hj /=".
-    smart_wp_bind (stlc_mu.lang.FstCtx) v v' "[Hv #Hiv]" ('`IHHtyped _ _ (FstCtx :: K)); cbn.
+    smart_wp_bind (cast_calculus.lang.FstCtx) v v' "[Hv #Hiv]" ('`IHHtyped _ _ (FstCtx :: K)); cbn.
     rewrite interp_rw_TProd.
     iDestruct "Hiv" as ([w1 w1'] [w2 w2']) "#[% [Hw1 Hw2]]"; simplify_eq.
     iMod (step_fst _ _ K (of_val w1') (of_val w2') with "[-]") as "Hw"; eauto.
@@ -83,10 +84,10 @@ Section fundamental.
 
   Lemma bin_log_related_snd Γ e e' τ1 τ2
       (IHHtyped : Γ ⊨ e ≤log≤ e' : TProd τ1 τ2) :
-    Γ ⊨ stlc_mu.lang.Snd e ≤log≤ Snd e' : τ2.
+    Γ ⊨ cast_calculus.lang.Snd e ≤log≤ Snd e' : τ2.
   Proof.
     iIntros (vvs ei') "#[Hρ HΓ]"; iIntros (K) "Hj /=".
-    smart_wp_bind (stlc_mu.lang.SndCtx) v v' "[Hv #Hiv]" ('`IHHtyped _ _ (SndCtx :: K)); cbn.
+    smart_wp_bind (cast_calculus.lang.SndCtx) v v' "[Hv #Hiv]" ('`IHHtyped _ _ (SndCtx :: K)); cbn.
     rewrite interp_rw_TProd.
     iDestruct "Hiv" as ([w1 w1'] [w2 w2']) "#[% [Hw1 Hw2]]"; simplify_eq.
     iMod (step_snd _ _ K (of_val w1') (of_val w2') with "[-]") as "Hw"; eauto.
@@ -95,10 +96,10 @@ Section fundamental.
 
   Lemma bin_log_related_injl Γ e e' τ1 τ2
       (IHHtyped : Γ ⊨ e ≤log≤ e' : τ1) :
-    Γ ⊨ stlc_mu.lang.InjL e ≤log≤ InjL e' : (TSum τ1 τ2).
+    Γ ⊨ cast_calculus.lang.InjL e ≤log≤ InjL e' : (TSum τ1 τ2).
   Proof.
     iIntros (vvs ei') "#[Hρ HΓ]"; iIntros (K) "Hj /=".
-    smart_wp_bind (stlc_mu.lang.InjLCtx) v v' "[Hv #Hiv]"
+    smart_wp_bind (cast_calculus.lang.InjLCtx) v v' "[Hv #Hiv]"
       ('`IHHtyped _ _ (InjLCtx :: K)); cbn.
     iApply wp_value. repeat rewrite /= to_of_val. eauto.
     iExists (InjLV v'); iFrame "Hv".
@@ -108,10 +109,10 @@ Section fundamental.
 
   Lemma bin_log_related_injr Γ e e' τ1 τ2
       (IHHtyped : Γ ⊨ e ≤log≤ e' : τ2) :
-    Γ ⊨ stlc_mu.lang.InjR e ≤log≤ InjR e' : TSum τ1 τ2.
+    Γ ⊨ cast_calculus.lang.InjR e ≤log≤ InjR e' : TSum τ1 τ2.
   Proof.
     iIntros (vvs ei') "#[Hρ HΓ]"; iIntros (K) "Hj /=".
-    smart_wp_bind (stlc_mu.lang.InjRCtx) v v' "[Hv #Hiv]"
+    smart_wp_bind (cast_calculus.lang.InjRCtx) v v' "[Hv #Hiv]"
       ('`IHHtyped _ _ (InjRCtx :: K)); cbn.
     iApply wp_value. repeat rewrite /= to_of_val. eauto.
     iExists (InjRV v'); iFrame "Hv".
@@ -119,15 +120,15 @@ Section fundamental.
     iRight; iExists (_,_); eauto 10.
   Qed.
 
-  Lemma bin_log_related_case Γ (e0 e1 e2 : stlc_mu.lang.expr) (e0' e1' e2' : cast_calculus.lang.expr) τ1 τ2 τ3
+  Lemma bin_log_related_case Γ (e0 e1 e2 : cast_calculus.lang.expr) (e0' e1' e2' : stlc_mu.lang.expr) τ1 τ2 τ3
       (IHHtyped1 : Γ ⊨ e0 ≤log≤ e0' : TSum τ1 τ2)
       (IHHtyped2 : τ1 :: Γ ⊨ e1 ≤log≤ e1' : τ3)
       (IHHtyped3 : τ2 :: Γ ⊨ e2 ≤log≤ e2' : τ3) :
-    Γ ⊨ stlc_mu.lang.Case e0 e1 e2 ≤log≤ Case e0' e1' e2' : τ3.
+    Γ ⊨ cast_calculus.lang.Case e0 e1 e2 ≤log≤ Case e0' e1' e2' : τ3.
   Proof.
     iIntros (vvs ei') "#[Hρ HΓ]"; iIntros (K) "Hj /=".
     iDestruct (interp_env_length with "HΓ") as %?.
-    smart_wp_bind (stlc_mu.lang.CaseCtx _ _) v v' "[Hv #Hiv]"
+    smart_wp_bind (cast_calculus.lang.CaseCtx _ _) v v' "[Hv #Hiv]"
       ('`IHHtyped1 _ _ ((CaseCtx _ _) :: K)); cbn.
     rewrite interp_rw_TSum.
     iDestruct "Hiv" as "[Hiv|Hiv]".
@@ -145,9 +146,9 @@ Section fundamental.
       iApply interp_env_cons; auto.
   Qed.
 
-  Lemma bin_log_related_lam Γ (e : stlc_mu.lang.expr) (e' : cast_calculus.lang.expr) τ1 τ2
+  Lemma bin_log_related_lam Γ (e : cast_calculus.lang.expr) (e' : stlc_mu.lang.expr) τ1 τ2
       (IHHtyped : τ1 :: Γ ⊨ e ≤log≤ e' : τ2) :
-    Γ ⊨ stlc_mu.lang.Lam e ≤log≤ Lam e' : TArrow τ1 τ2.
+    Γ ⊨ cast_calculus.lang.Lam e ≤log≤ Lam e' : TArrow τ1 τ2.
   Proof.
     iIntros (vvs ei') "#[Hρ HΓ]"; iIntros (K) "Hj /=".
     iApply wp_value. iExists (LamV _).
@@ -164,12 +165,12 @@ Section fundamental.
   Lemma bin_log_related_app Γ e1 e2 e1' e2' τ1 τ2
       (IHHtyped1 : Γ ⊨ e1 ≤log≤ e1' : TArrow τ1 τ2)
       (IHHtyped2 : Γ ⊨ e2 ≤log≤ e2' : τ1) :
-    Γ ⊨ stlc_mu.lang.App e1 e2 ≤log≤ App e1' e2' :  τ2.
+    Γ ⊨ cast_calculus.lang.App e1 e2 ≤log≤ App e1' e2' :  τ2.
   Proof.
     iIntros (vvs ei') "#[Hρ HΓ]"; iIntros (K) "Hj /=".
-    smart_wp_bind (stlc_mu.lang.AppLCtx (e2.[stlc_mu.typing.env_subst (vvs.*1)])) v v' "[Hv #Hiv]"
-      ('`IHHtyped1 _ _ (((AppLCtx (e2'.[env_subst (vvs.*2)]))) :: K)); cbn.
-    smart_wp_bind (stlc_mu.lang.AppRCtx v) w w' "[Hw #Hiw]"
+    smart_wp_bind (cast_calculus.lang.AppLCtx (e2.[cast_calculus.typing.env_subst (vvs.*1)])) v v' "[Hv #Hiv]"
+      ('`IHHtyped1 _ _ (((AppLCtx (e2'.[_]))) :: K)); cbn.
+    smart_wp_bind (cast_calculus.lang.AppRCtx v) w w' "[Hw #Hiw]"
                   ('`IHHtyped2 _ _ ((AppRCtx v') :: K)); cbn.
     rewrite interp_rw_TArrow.
     iApply ("Hiv" $! (w, w') with "Hiw"); simpl; eauto.
@@ -177,10 +178,10 @@ Section fundamental.
 
   Lemma bin_log_related_fold Γ e e' τ
       (IHHtyped : Γ ⊨ e ≤log≤ e' : τ.[(TRec τ)/]) :
-    Γ ⊨ stlc_mu.lang.Fold e ≤log≤ cast_calculus.lang.Fold e' : TRec τ.
+    Γ ⊨ cast_calculus.lang.Fold e ≤log≤ stlc_mu.lang.Fold e' : TRec τ.
   Proof.
     iIntros (vvs ei') "#[Hρ HΓ]"; iIntros (K) "Hj /=".
-    iApply (wp_bind (stlc_mu.lang.fill_item stlc_mu.lang.FoldCtx)).
+    iApply (wp_bind [cast_calculus.lang.FoldCtx]).
     iApply (wp_wand with "[Hj]"). iApply ('`IHHtyped _ _ (FoldCtx :: K)). iFrame. auto.
     iIntros (v); iDestruct 1 as (v') "[Hv #Hiv]".
     iApply wp_value.
@@ -191,10 +192,10 @@ Section fundamental.
 
   Lemma bin_log_related_unfold Γ e e' τ
       (IHHtyped : Γ ⊨ e ≤log≤ e' : TRec τ) :
-    Γ ⊨ stlc_mu.lang.Unfold e ≤log≤ Unfold e' : τ.[(TRec τ)/].
+    Γ ⊨ cast_calculus.lang.Unfold e ≤log≤ Unfold e' : τ.[(TRec τ)/].
   Proof.
     iIntros (vvs ei') "#[Hρ HΓ]"; iIntros (K) "Hj /=".
-    iApply (wp_bind (stlc_mu.lang.fill_item stlc_mu.lang.UnfoldCtx)).
+    iApply (wp_bind [cast_calculus.lang.UnfoldCtx]).
     iApply (wp_wand with "[Hj]"). iApply ('`IHHtyped _ _ (UnfoldCtx :: K)). iFrame. auto.
     iIntros (v). iDestruct 1 as (v') "[Hw #Hiw]".
     simpl.
@@ -204,6 +205,5 @@ Section fundamental.
     iApply wp_pure_step_later; cbn; auto.
     iNext. iApply wp_value; auto.
   Qed.
-
 
 End fundamental.
