theories/refinements/gradual_static/logical_relation.v
@@ -1,0 +1,237 @@
+From iris.proofmode Require Import tactics.
+From iris.program_logic Require Export weakestpre.
+From iris.base_logic Require Export invariants.
+From fae_gtlc_mu.backtranslation.cast_help Require Export embed.
+From fae_gtlc_mu.refinements Require Export prelude.
+From fae_gtlc_mu.refinements.gradual_static Require Export resources_left resources_right.
+From fae_gtlc_mu.cast_calculus Require Export types lang.
+From iris.algebra Require Import list ofe.
+From stdpp Require Import tactics.
+Import uPred.
+
+Canonical Structure typeO := leibnizO type.
+
+(* HACK: move somewhere else *)
+Ltac auto_equiv :=
+  (* Deal with "pointwise_relation" *)
+  repeat lazymatch goal with
+  | |- pointwise_relation _ _ _ _ => intros ?
+  end;
+  (* Normalize away equalities. *)
+  repeat match goal with
+  | H : _ ≡{_}≡ _ |-  _ => apply (discrete_iff _ _) in H
+  | _ => progress simplify_eq
+  end;
+  (* repeatedly apply congruence lemmas and use the equalities in the hypotheses. *)
+  try (f_equiv; fast_done || auto_equiv).
+
+Definition logN : namespace := nroot .@ "logN".
+
+(** interp : is a binary logical relation. *)
+Section logrel.
+  Context `{!implG Σ, !specG Σ}.
+  Notation P := (prodO cast_calculus.lang.valO stlc_mu.lang.valO).
+  Notation D := (prodO cast_calculus.lang.valO stlc_mu.lang.valO -n> iPropO Σ).
+  Implicit Types τi : D.
+  Implicit Types Δ : listO D.
+
+  Definition castupV_TUnit (v : val) : val :=
+    (CastV v TUnit ⋆ (TGround_TUnknown_icp Ground_TUnit)).
+
+  Definition castupV_TSum (v : val) : val :=
+    (CastV v (TSum ⋆ ⋆) ⋆ (TGround_TUnknown_icp Ground_TSum)).
+
+  Definition castupV_TProd (v : val) : val :=
+    (CastV v (TProd ⋆ ⋆) ⋆ (TGround_TUnknown_icp Ground_TProd)).
+
+  Definition castupV_TArrow (v : val) : val :=
+    (CastV v (TArrow ⋆ ⋆) ⋆ (TGround_TUnknown_icp Ground_TArrow)).
+
+  Definition castupV_TRec (v : val) : val :=
+    (CastV v (TRec ⋆) ⋆ (TGround_TUnknown_icp Ground_TRec)).
+
+  From fae_gtlc_mu.stlc_mu Require Export lang.
+
+  Definition interp_expr (interp_cor_val : P → iPropO Σ)
+      (ee : cast_calculus.lang.expr * stlc_mu.lang.expr) : iProp Σ := (∀ K',
+    currently_half (fill K' (ee.2)) →
+    WP ee.1 ?{{ v, ∃ v', currently_half (fill K' (of_val v')) ∗ interp_cor_val (v, v') }})%I.
+
+  Definition TClosed (τ : type) : Prop := forall σ, τ.[σ] = τ.
+
+  (** only to be used with closed types *)
+
+  Fixpoint interp_gen (Ψ : typeO -n> D) (τ : typeO) (ww : P) : iPropO Σ := (
+    match τ with
+    | TUnit => ⌜ww.1 = cast_calculus.lang.UnitV⌝ ∧ ⌜ww.2 = stlc_mu.lang.UnitV⌝
+    | TProd τ1 τ2 => ∃ v1v1' v2v2', ⌜ww = (cast_calculus.lang.PairV (v1v1'.1) (v2v2'.1), stlc_mu.lang.PairV (v1v1'.2) (v2v2'.2))⌝ ∧
+                                  interp_gen Ψ τ1 v1v1' ∧ interp_gen Ψ τ2 v2v2'
+    | TSum τ1 τ2 => (∃ vv', ⌜ww = (cast_calculus.lang.InjLV (vv'.1), InjLV (vv'.2))⌝ ∧ interp_gen Ψ τ1 vv') ∨
+                    (∃ vv', ⌜ww = (cast_calculus.lang.InjRV (vv'.1), InjRV (vv'.2))⌝ ∧ interp_gen Ψ τ2 vv')
+    | TArrow τ1 τ2 => □ ∀ vv, interp_gen Ψ τ1 vv →
+             interp_expr
+               (interp_gen Ψ τ2) (cast_calculus.lang.App (cast_calculus.lang.of_val (ww.1)) (cast_calculus.lang.of_val (vv.1)),
+                        stlc_mu.lang.App (stlc_mu.lang.of_val (ww.2)) (stlc_mu.lang.of_val (vv.2)))
+    | TRec τb => □ ∃ w w', ⌜ww = (cast_calculus.lang.FoldV w, stlc_mu.lang.FoldV w')⌝ ∧ ▷ Ψ (τb.[TRec τb/]) (w, w')
+    | TUnknown => ∃ v v', □ (
+                               (⌜ ww = (castupV_TUnit v , embedV_TUnit v') ⌝                   ∧ ▷ Ψ TUnit (v, v') )
+                             ∨ (⌜ ww = (castupV_TProd v, embedV_Ground_TProd v') ⌝            ∧ ▷ Ψ (TProd TUnknown TUnknown) (v , v'))
+                             ∨ (⌜ ww = (castupV_TSum v , embedV_Ground_TSum v') ⌝              ∧ ▷ Ψ (TSum TUnknown TUnknown) (v , v'))
+                             ∨ (⌜ ww = (castupV_TArrow v , embedV_Ground_TArrow v') ⌝          ∧ ▷ Ψ (TArrow TUnknown TUnknown) (v , v'))
+                             ∨ (⌜ ww = (castupV_TRec (cast_calculus.lang.FoldV v), embedV_TUnknown v') ⌝ ∧ ▷ Ψ TUnknown (v , v')
+                             (* ∨ (∃ u u', ⌜ ww = (embedV_TUnknown u, castupV_TRec (FoldV u')) ⌝ ∧ ▷ Ψ TUnknown (u , u') *)
+                               )
+      )
+    | TVar x => False (** exfaslo ... *)
+    end)%I.
+
+  Program Definition interp_gen_ne (Ψ : typeO -n> D) : typeO -n> D := λne τ p, interp_gen Ψ τ p.
+  Solve Obligations with repeat intros ?; simpl; auto_equiv.
+
+  Global Instance interp_gen_ne_contractive : Contractive interp_gen_ne.
+  Proof.
+    intros n Ψ1 Ψ2  pnΨ τ. simpl.
+    induction τ; intro p; simpl.
+    - auto.
+    - f_equiv. intro p1. f_equiv. intro p2. f_equiv. f_equiv.
+      + exact (IHτ1 p1).
+      + exact (IHτ2 p2).
+    - f_equiv.
+      + f_equiv. intro a. f_equiv. exact (IHτ1 a).
+      + f_equiv. intro a. f_equiv. exact (IHτ2 a).
+    - f_equiv. f_equiv. intro. f_equiv.
+      + exact (IHτ1 a).
+      + rewrite /interp_expr. simpl. f_equiv. intro K.
+        f_equiv. f_equiv. intro v. f_equiv. intro v'.
+        f_equiv. exact (IHτ2 (v, v')).
+    - solve_contractive.
+    - solve_contractive.
+    - solve_contractive.
+  Qed.
+
+  Definition interp : typeO -n> D := fixpoint interp_gen_ne.
+
+  Notation "⟦ τ ⟧" := (interp τ). (** the actual relations on values *)
+
+  (* boring lemma's related to foldings {{{ *)
+
+  Lemma unfold_interp : interp ≡ interp_gen_ne interp.
+  Proof. apply fixpoint_unfold. Qed.
+
+  Lemma unfold_interp_type τ : interp τ ≡ interp_gen_ne interp τ.
+  Proof. f_equiv. apply unfold_interp. Qed.
+
+  Lemma unfold_interp_type_pair τ vv : interp τ vv ≡ interp_gen interp τ vv.
+  Proof. assert (H : interp_gen interp τ vv ≡ interp_gen_ne interp τ vv). auto_equiv. rewrite H. apply unfold_interp_type. Qed.
+
+  Lemma interp_rw_TUnit ww : interp TUnit ww ≡
+    (⌜ww.1 = cast_calculus.lang.UnitV⌝ ∧ ⌜ww.2 = stlc_mu.lang.UnitV⌝)%I.
+  Proof. by rewrite (unfold_interp_type_pair TUnit). Qed.
+
+  Lemma interp_rw_TProd τ1 τ2 ww : interp (TProd τ1 τ2) ww ≡
+    (∃ v1v1' v2v2', ⌜ww = (cast_calculus.lang.PairV (v1v1'.1) (v2v2'.1), stlc_mu.lang.PairV (v1v1'.2) (v2v2'.2))⌝ ∧
+                                  interp τ1 v1v1' ∧ interp τ2 v2v2')%I.
+  Proof. rewrite (unfold_interp_type_pair (TProd τ1 τ2)). simpl. auto_equiv; by rewrite -unfold_interp_type_pair. Qed.
+
+  Lemma interp_rw_TSum τ1 τ2 ww : interp (TSum τ1 τ2) ww ≡
+    ((∃ vv', ⌜ww = (cast_calculus.lang.InjLV (vv'.1), InjLV (vv'.2))⌝ ∧ interp τ1 vv') ∨
+                    (∃ vv', ⌜ww = (cast_calculus.lang.InjRV (vv'.1), InjRV (vv'.2))⌝ ∧ interp τ2 vv'))%I.
+  Proof. rewrite (unfold_interp_type_pair (TSum τ1 τ2)). simpl. auto_equiv; by rewrite -unfold_interp_type_pair. Qed.
+
+  Lemma interp_gen_interp_gen_ne Ψ τ ww : interp_gen Ψ τ ww ≡ interp_gen_ne Ψ τ ww.
+  Proof. auto. Qed.
+
+  Lemma interp_rw_TArrow τ1 τ2 ww : interp (TArrow τ1 τ2) ww ≡
+    (□ ∀ vv, interp τ1 vv →
+             interp_expr
+               (interp τ2) (cast_calculus.lang.App (cast_calculus.lang.of_val (ww.1)) (cast_calculus.lang.of_val (vv.1)),
+                        stlc_mu.lang.App (stlc_mu.lang.of_val (ww.2)) (stlc_mu.lang.of_val (vv.2))))%I.
+  Proof. rewrite (unfold_interp_type_pair (TArrow τ1 τ2)). simpl.
+         f_equiv. f_equiv.  intro. f_equiv. by rewrite -unfold_interp_type_pair.
+         rewrite /interp_expr. auto_equiv. by rewrite unfold_interp_type_pair.
+  Qed.
+
+  Lemma interp_rw_TRec τb ww : interp (TRec τb) ww ≡
+    (□ ∃ w w', ⌜ww = (cast_calculus.lang.FoldV w, stlc_mu.lang.FoldV w')⌝ ∧ ▷ interp (τb.[TRec τb/]) (w, w'))%I.
+  Proof. rewrite (unfold_interp_type_pair). by simpl. Qed.
+
+  Lemma interp_rw_TUnknown ww : interp TUnknown ww ≡
+    (∃ v v', □ (
+                 (⌜ ww = (castupV_TUnit v , embedV_TUnit v') ⌝                   ∧ ▷ interp TUnit (v, v') )
+                 ∨ (⌜ ww = (castupV_TProd v, embedV_Ground_TProd v') ⌝            ∧ ▷ interp (TProd TUnknown TUnknown) (v , v'))
+                 ∨ (⌜ ww = (castupV_TSum v , embedV_Ground_TSum v') ⌝              ∧ ▷ interp (TSum TUnknown TUnknown) (v , v'))
+                 ∨ (⌜ ww = (castupV_TArrow v , embedV_Ground_TArrow v') ⌝          ∧ ▷ interp (TArrow TUnknown TUnknown) (v , v'))
+                 ∨ (⌜ ww = (castupV_TRec (cast_calculus.lang.FoldV v), embedV_TUnknown v') ⌝ ∧ ▷ interp TUnknown (v , v')
+                   )
+      ))%I.
+  Proof. rewrite (unfold_interp_type_pair). by simpl. Qed.
+
+  (* }}} *)
+
+  Global Instance interp_persistent τ vv :
+    Persistent (⟦ τ ⟧ vv).
+  Proof.
+    revert vv. induction τ; intro p; rewrite unfold_interp_type_pair; simpl; try by apply _.
+    - apply exist_persistent. intro q. apply exist_persistent. intro r.
+      do 2 rewrite -unfold_interp_type_pair. apply _.
+    - apply or_persistent; apply exist_persistent; intro q; rewrite -unfold_interp_type_pair; apply _.
+  Qed.
+
+
+  Definition interp_env (Γ : list type)
+      (vvs : list (cast_calculus.lang.val * stlc_mu.lang.val)) : iProp Σ :=
+    (⌜length Γ = length vvs⌝ ∗ [∗] zip_with (λ τ, ⟦ τ ⟧) Γ vvs)%I.
+  Notation "⟦ Γ ⟧*" := (interp_env Γ).
+
+  Global Instance interp_env_base_persistent Γ vs :
+  TCForall Persistent (zip_with (λ τ, ⟦ τ ⟧) Γ vs).
+  Proof.
+    revert vs.
+    induction Γ => vs; simpl; destruct vs; constructor; apply _.
+  Qed.
+  Global Instance interp_env_persistent Γ vvs :
+    Persistent (⟦ Γ ⟧* vvs) := _.
+
+  Lemma interp_env_length Γ vvs : ⟦ Γ ⟧* vvs ⊢ ⌜length Γ = length vvs⌝.
+  Proof. by iIntros "[% ?]". Qed.
+
+  Lemma interp_env_Some_l Γ vvs x τ :
+    Γ !! x = Some τ → ⟦ Γ ⟧* vvs ⊢ (∃ vv, ⌜vvs !! x = Some vv⌝ ∧ ⟦ τ ⟧ vv).
+  Proof.
+    iIntros (?) "[Hlen HΓ]"; iDestruct "Hlen" as %Hlen.
+    destruct (lookup_lt_is_Some_2 vvs x) as [v Hv].
+    { by rewrite -Hlen; apply lookup_lt_Some with τ. }
+    iExists v; iSplit. done. iApply (big_sepL_elem_of with "HΓ").
+    apply elem_of_list_lookup_2 with x.
+    rewrite lookup_zip_with; by simplify_option_eq.
+  Qed.
+
+  Lemma interp_env_nil : ⊢ ⟦ [] ⟧* [].
+  Proof. iSplit; simpl; auto. Qed.
+  Lemma interp_env_cons Γ vvs τ vv :
+    ⟦ τ :: Γ ⟧* (vv :: vvs) ⊣⊢ ⟦ τ ⟧ vv ∗ ⟦ Γ ⟧* vvs.
+  Proof.
+    rewrite /interp_env /= (assoc _ (⟦ _ ⟧ _)) -(comm _ ⌜_ = _⌝%I) -assoc.
+    by apply sep_proper; [apply pure_proper; lia|].
+  Qed.
+
+End logrel.
+
+Typeclasses Opaque interp_env.
+Notation "⟦ τ ⟧" := (interp τ).
+Notation "⟦ τ ⟧ₑ" := (interp_expr (interp τ)).
+Notation "⟦ Γ ⟧*" := (interp_env Γ).
+
+From fae_gtlc_mu.stlc_mu Require Export types typing.
+From fae_gtlc_mu.cast_calculus Require Export types typing.
+
+Section bin_log_def.
+  Context `{!implG Σ, !specG Σ}.
+  Notation D := (prodO cast_calculus.lang.valO stlc_mu.lang.valO -n> iProp Σ).
+
+  Definition bin_log_related
+  (Γ : list cast_calculus.types.type) (e : cast_calculus.lang.expr) (e' : stlc_mu.lang.expr) (τ : cast_calculus.types.type) :=
+    ∀ vvs (ei' : stlc_mu.lang.expr),
+    initially_inv ei' ∗ ⟦ Γ ⟧* vvs ⊢
+    ⟦ τ ⟧ₑ (e.[cast_calculus.typing.env_subst (vvs.*1)], e'.[stlc_mu.typing.env_subst (vvs.*2)]).
+End bin_log_def.
