theories/refinements/gradual_static/resources_left.v
@@ -1,0 +1,256 @@
+From iris.program_logic Require Import lifting.
+From iris.program_logic Require Export weakestpre.
+From iris.base_logic Require Export invariants.
+From iris.algebra Require Import auth frac agree gmap.
+From iris.proofmode Require Import tactics.
+From iris.base_logic Require Export gen_heap.
+From iris.program_logic Require Import language.
+From fae_gtlc_mu.cast_calculus Require Export lang lang_props.
+Import uPred.
+
+Class implG Σ := ImplG { (* resources for the implementation side *)
+  implG_invG : invG Σ; (* for fancy updates, invariants... *)
+}.
+
+Instance implG_irisG `{implG Σ} : irisG lang Σ := {
+  iris_invG := implG_invG;
+  state_interp σ κs _ := True%I;
+  fork_post _ := True%I;
+}.
+Global Opaque iris_invG.
+
+Section lang_rules.
+  Context `{implG Σ}.
+  Implicit Types P Q : iProp Σ.
+  Implicit Types Φ : cast_calculus.lang.val → iProp Σ.
+  (* Implicit Types σ : state. *)
+  Implicit Types e : cast_calculus.lang.expr.
+
+  (** The tactic [inv_head_step] performs inversion on hypotheses of the shape
+      [head_step]. The tactic will discharge head-reductions starting from values, and
+      simplifies hypothesis related to conversions from and to values, and finite map
+      operations. This tactic is slightly ad-hoc and tuned for proving our lifting
+      lemmas. *)
+  Ltac inv_head_step :=
+    repeat match goal with
+    | _ => progress simplify_map_eq/= (* simplify memory stuff *)
+    | H : to_val _ = Some _ |- _ => apply of_to_val in H
+    | H : head_step ?e _ _ _ _ _ |- _ =>
+       try (is_var e; fail 1); (* inversion yields many goals if [e] is a variable
+       and can thus better be avoided. *)
+       inversion H; subst; clear H
+    end.
+
+  Local Hint Extern 0 (head_reducible _ _) => eexists _, _, _, _; simpl : core.
+
+  Local Hint Constructors head_step : core.
+  (* Local Hint Resolve alloc_fresh : core. *)
+  Local Hint Resolve to_of_val : core.
+
+  Local Ltac solve_exec_safe := intros; subst; do 3 eexists; econstructor; eauto.
+  Local Ltac solve_exec_puredet := simpl; intros; by inv_head_step.
+  Local Ltac solve_pure_exec :=
+    unfold IntoVal in *;
+    repeat match goal with H : AsVal _ |- _ => destruct H as [??] end; subst;
+    intros ?; apply nsteps_once, pure_head_step_pure_step;
+      constructor; [solve_exec_safe | solve_exec_puredet].
+
+
+
+
+  (** We want to have another bind operator.
+      Why? Our contexts are not evaluation contexts anymore *)
+
+
+  Lemma wp_CastError' E Φ :
+    ⊢ WP CastError @ MaybeStuck; E {{Φ}}.
+  Proof. simpl. iApply wp_lift_pure_stuck. intro σ. destruct σ. exact CastError_stuck. done. Qed.
+
+  Lemma wp_CastError (K : ectx) E Φ :
+    ⊢ WP fill K CastError @ MaybeStuck; E {{Φ}}.
+  Proof.
+    destruct K.
+    - by iApply wp_CastError'.
+    - iApply (wp_pure_step_later MaybeStuck _ _ CastError True 1 _).
+      intros _. apply nsteps_once. by apply cast_error_step. done.
+      iApply wp_lift_pure_stuck. intro σ. destruct σ. exact CastError_stuck. done.
+  Qed.
+
+  Lemma wp_bind (K : ectx) E e Φ :
+    WP e @ MaybeStuck; E {{ v, WP fill K (of_val v) @ MaybeStuck; E {{ Φ }} }} ⊢ WP fill K e @ MaybeStuck; E {{ Φ }}.
+  Proof.
+    destruct (decide (e = CastError)) as [-> | eNeqCE].
+    { iIntros "_". iApply wp_CastError. }
+    iIntros "H". iLöb as "IH" forall (E e eNeqCE Φ). rewrite wp_unfold /wp_pre.
+    assert (language.to_val e = to_val e) as ->; first done.
+    destruct (to_val e) as [v|] eqn:He.
+    { apply of_to_val in He as <-. by iApply fupd_wp. }
+    rewrite wp_unfold /wp_pre.
+    assert (language.to_val (fill K  e) = to_val (fill K e)) as ->; first done.
+    rewrite fill_not_val //.
+    iIntros (σ1 κ κs n) "Hσ". iMod ("H" $! tt [] [] 0 with "[$]") as "[% H]". iModIntro; iSplit.
+    { eauto using reducible_fill. }
+    iIntros (e2 σ2 efs Hstep).
+    destruct (decide (e2 = CastError)).
+    - rewrite e0.
+      iMod ("H" $! CastError σ2 efs with "[]") as "H".
+      simpl. iPureIntro. cut (prim_step e [] CastError []). inversion Hstep; done.
+      { assert (prim_step (fill K e) [] e2 []). inversion Hstep; simplify_eq; by econstructor. eapply fill_step_CastError_inv; eauto. by simplify_eq. }
+      iIntros "!>!>".
+      iMod "H" as "(Hσ' & H & Hefs)".
+      iModIntro. iFrame "Hσ Hefs". assert (CastError = fill [] CastError) as ->. done. iApply wp_CastError.
+    - destruct (fill_step_inv K e κ e2 efs) as (e2'&->&?); auto.
+      iMod ("H" $! e2' σ2 efs with "[]") as "H".
+      simpl. inversion H1; by simplify_eq.
+      iIntros "!>!>".
+      iMod "H" as "(Hσ' & H & Hefs)".
+      iModIntro. iFrame "Hσ Hefs".
+      destruct K as [|Ki K]. simpl. iApply wp_fupd. iApply (wp_wand with "H"). iIntros (v) "Hwpv". iMod (wp_value_inv with "Hwpv"). by iModIntro.
+      destruct (decide (e2' = CastError)) as [-> | neq]. iApply wp_CastError.
+      by iApply "IH".
+  Qed.
+
+
+
+  Global Instance pure_lam e1 e2 `{!AsVal e2} :
+    PureExec True 1 (App (Lam e1) e2) e1.[e2 /].
+  Proof.
+    intros _. apply nsteps_once. apply prim_step_pure.
+    destruct AsVal0 as [??];subst.
+    eapply (Ectx_step []); eauto.
+  Qed.
+
+  (* Global Instance pure_tlam e : PureExec True 1 (TApp (TLam e)) e. *)
+  (* Proof. solve_pure_exec. Qed. *)
+
+  Global Instance pure_fold e `{!AsVal e}:
+    PureExec True 1 (Unfold (Fold e)) e.
+  Proof.
+    intros _. apply nsteps_once. apply prim_step_pure.
+    destruct AsVal0 as [??];subst.
+    eapply (Ectx_step []); eauto.
+  Qed.
+
+  Global Instance pure_fst e1 e2 `{!AsVal e1, !AsVal e2} :
+    PureExec True 1 (Fst (Pair e1 e2)) e1.
+  Proof.
+    intros _. apply nsteps_once. apply prim_step_pure.
+    destruct AsVal0 as [??];subst.
+    destruct AsVal1 as [??];subst.
+    eapply (Ectx_step []); eauto.
+  Qed.
+  Proof.
+  (* Proof. solve_pure_exec. Qed. *)
+
+  Global Instance pure_snd e1 e2 `{!AsVal e1, !AsVal e2} :
+    PureExec True 1 (Snd (Pair e1 e2)) e2.
+  Proof.
+    intros _. apply nsteps_once. apply prim_step_pure.
+    destruct AsVal0 as [??];subst.
+    destruct AsVal1 as [??];subst.
+    eapply (Ectx_step []); eauto.
+  Qed.
+
+  Global Instance pure_case_inl e0 e1 e2 `{!AsVal e0}:
+    PureExec True 1 (Case (InjL e0) e1 e2) e1.[e0/].
+  Proof.
+    intros _. apply nsteps_once. apply prim_step_pure.
+    destruct AsVal0 as [??];subst.
+    eapply (Ectx_step []); eauto.
+  Qed.
+
+  Global Instance pure_case_inr e0 e1 e2 `{!AsVal e0}:
+    PureExec True 1 (Case (InjR e0) e1 e2) e2.[e0/].
+  Proof.
+    intros _. apply nsteps_once. apply prim_step_pure.
+    destruct AsVal0 as [??];subst.
+    eapply (Ectx_step []); eauto.
+  Qed.
+
+  Global Instance pure_cast_between_sum e τ1 τ2 τ1' τ2' `{!AsVal e}:
+    PureExec True 1 (Cast e (TSum τ1 τ2) (TSum τ1' τ2')) (Case e (InjL (Cast (Var 0) τ1 τ1')) (InjR (Cast (Var 0) τ2 τ2'))).
+  Proof.
+    intros _. apply nsteps_once. apply prim_step_pure.
+    destruct AsVal0 as [??];subst.
+    eapply (Ectx_step []); eauto.
+  Qed.
+
+  Global Instance pure_cast_between_rec e τl τr `{!AsVal e}:
+    PureExec True 1 (Cast e (TRec τl) (TRec τr))
+             (Fold (Cast (Unfold e) τl.[TRec τl/] τr.[TRec τr/])).
+  Proof.
+    intros _. apply nsteps_once. apply prim_step_pure.
+    destruct AsVal0 as [??];subst.
+    eapply (Ectx_step []); eauto.
+  Qed.
+
+  Global Instance pure_app_cast f e2 τ1 τ2 τ1' τ2' `{!AsVal f,!AsVal e2} :
+    PureExec True 1 (App (Cast f (TArrow τ1 τ2) (TArrow τ1' τ2')) e2) (Cast (App f (Cast e2 τ1' τ1)) τ2 τ2').
+  Proof.
+    intros _. apply nsteps_once. apply prim_step_pure.
+    destruct AsVal0 as [??];subst.
+    destruct AsVal1 as [??];subst.
+    eapply (Ectx_step []); eauto.
+  Qed.
+
+  Global Instance pure_same_ground e τ `{!AsVal e, !Ground τ} :
+    PureExec True 1 (Cast (Cast e τ ⋆) ⋆ τ) e.
+  Proof.
+    intros _. apply nsteps_once. apply prim_step_pure.
+    destruct AsVal0 as [??];subst.
+    eapply (Ectx_step []); eauto.
+  Qed.
+
+  Global Instance pure_different_ground e τ τ' (neq : τ ≠ τ') `{!AsVal e, !Ground τ, !Ground τ'} :
+    PureExec True 1 (Cast (Cast e τ ⋆) ⋆ τ') CastError.
+  Proof.
+    intros _. apply nsteps_once. apply prim_step_pure.
+    destruct AsVal0 as [??];subst.
+    eapply (Ectx_step []); eauto.
+  Qed.
+
+  Lemma pure_fact_up e τ τG (neq : τ ≠ ⋆) (nG : Ground τ → False) (G : get_shape τ = Some τG) `{!AsVal e} :
+    PureExec True 1 (Cast e τ ⋆) (Cast (Cast e τ τG) τG ⋆).
+  Proof.
+    intros _. apply nsteps_once. apply prim_step_pure.
+    destruct AsVal0 as [??];subst.
+    eapply (Ectx_step []); eauto.
+  Qed.
+
+  Lemma pure_fact_down e τ τG (neq : τ ≠ ⋆) (nG : Ground τ → False) (G : get_shape τ = Some τG) `{!AsVal e} :
+    PureExec True 1 (Cast e ⋆ τ) (Cast (Cast e ⋆ τG) τG τ).
+  Proof.
+    intros _. apply nsteps_once. apply prim_step_pure.
+    destruct AsVal0 as [??];subst.
+    eapply (Ectx_step []); eauto.
+  Qed.
+
+  Global Instance pure_cast_pair e τ1 τ2 τ1' τ2' `{!AsVal e} :
+    PureExec True 1 (Cast e (TProd τ1 τ2) (TProd τ1' τ2')) (Pair (Cast (Fst e) τ1 τ1') (Cast (Snd e) τ2 τ2')).
+  Proof.
+    intros _. apply nsteps_once. apply prim_step_pure.
+    destruct AsVal0 as [??];subst.
+    eapply (Ectx_step []); eauto.
+  Qed.
+
+  Global Instance pure_cast_tunit_tunit e  `{!AsVal e} :
+    PureExec True 1 (Cast e TUnit TUnit) e.
+  Proof.
+    intros _. apply nsteps_once. apply prim_step_pure.
+    destruct AsVal0 as [??];subst.
+    eapply (Ectx_step []); eauto.
+  Qed.
+
+  Global Instance pure_cast_tunk_tunk e  `{!AsVal e} :
+    PureExec True 1 (Cast e ⋆ ⋆) e.
+  Proof.
+    intros _. apply nsteps_once. apply prim_step_pure.
+    destruct AsVal0 as [??];subst.
+    eapply (Ectx_step []); eauto.
+  Qed.
+
+End lang_rules.
+
+Ltac wp_head := iApply wp_pure_step_later; auto; iNext.
+Ltac wp_value := iApply wp_value.
+
