theories/refinements/gradual_static/resources_right.v
@@ -1,8 +1,8 @@
 From iris.algebra Require Import cmra excl auth frac agree gmap list.
 From iris.program_logic Require Import lifting.
 From iris.proofmode Require Import tactics.
-From fae_gtlc_mu.refinements.static_gradual Require Export resources_left.
-From fae_gtlc_mu.cast_calculus Require Export lang.
+From fae_gtlc_mu.refinements.gradual_static Require Export resources_left.
+From fae_gtlc_mu.stlc_mu Require Export lang.
 Import uPred.
 
 Definition specN := nroot .@ "gradual".
@@ -29,26 +29,6 @@ Definition initially_body `{specG Σ} (ei' : expr) : iProp Σ :=
 Definition initially_inv `{specG Σ} `{invG Σ} (ei' : expr) : iProp Σ :=
   inv specN (initially_body ei').
 
-(* Section definitionsS. *)
-  (* Context `{specG Σ}. *)
-
-  (* Definition heapS_mapsto (l : loc) (q : Qp) (v: val) : iProp Σ := *)
-    (* own cfg_name (◯ (ε, {[ l := (q, to_agree v) ]})). *)
-
-  (* Definition tpool_mapsto (e: expr) : iProp Σ := *)
-    (* own cfg_name (◯ (Excl' e, ∅)). *)
-
-  (* Global Instance heapS_mapsto_timeless l q v : Timeless (heapS_mapsto l q v). *)
-  (* Proof. apply _. Qed. *)
-(* End definitionsS. *)
-
-(* Typeclasses Opaque heapS_mapsto tpool_mapsto. *)
-
-(* Notation "l ↦ₛ{ q } v" := (heapS_mapsto l q v) *)
-  (* (at level 20, q at level 50, format "l  ↦ₛ{ q }  v") : bi_scope. *)
-(* Notation "l ↦ₛ v" := (heapS_mapsto l 1 v) (at level 20) : bi_scope. *)
-(* Notation "⤇ e" := (tpool_mapsto e) (at level 20) : bi_scope. *)
-
 Section cfg.
   Context `{!specG Σ}.
   Context `{!invG Σ}.
@@ -62,14 +42,14 @@ Section cfg.
 
   (** Conversion to tpools and back *)
   Lemma step_insert_no_fork K e σ e' σ' :
-    head_step e e' → erased_step ([fill K e], σ) ([fill K e'], σ').
+    head_step e σ [] e' σ' [] → erased_step ([fill K e], σ) ([fill K e'], σ').
   Proof. intros Hst. exists []. eapply (step_atomic _ _ _ _ _ _ _ [] [] []); eauto.
          by apply: Ectx_step.
   Qed.
 
   Local Set Warnings "-notation-overridden".
-  Lemma step_pure E ei' K e1' e2' :
-    (head_step e1' e2') →
+  Lemma step_pure E ei' K e1' e2' σ :
+    (head_step e1' σ [] e2' σ []) →
     nclose specN ⊆ E →
     initially_inv ei' ∗ currently_half (fill K e1') ={E}=∗ currently_half (fill K e2').
   Proof.
@@ -99,40 +79,106 @@ Section cfg.
     iNext. iExists (fill K e2'). iFrame.
     iPureIntro.
     eapply rtc_r, step_insert_no_fork; eauto.
-    iIntros (_). done.
+    destruct σ. by simpl in H. iFrame "Hown2". done.
+  Qed.
+
+  Lemma nsteps_pure_step_ctx n e1' e2' K :
+    nsteps pure_step n e1' e2' → nsteps pure_step n (fill K e1') (fill K e2').
+  Proof.
+    revert e2'. revert e1'.
+    induction n.
+    - intros e1 e2 H. inversion H. simplify_eq. constructor.
+    - intros e1 e2 H. inversion H. econstructor.
+      SearchAbout pure_step.
+      apply pure_step_ctx.
+      apply hack. apply H1. by apply IHn.
+  Qed.
+
+  Lemma pure_step_prim_step e e' : pure_step e e' → prim_step e tt [] e' tt [].
+    intro Pstp. destruct Pstp. destruct (pure_step_safe tt).
+    destruct H as [σ [ls Hprim]]. destruct σ.
+    by destruct (pure_step_det tt [] x tt ls Hprim) as [_ [ _ [-> ->]]].
+  Qed.
+
+  Lemma pure_step_erased_step e e' : pure_step e e' → erased_step ([e], ()) ([e'],()).
+  Proof. intros Pst. exists []. eapply (step_atomic _ _ _ _ _ _ _ [] [] []); eauto. by apply pure_step_prim_step. Qed.
+
+  Lemma nsteps_pure_step_prim_step n e e' : nsteps pure_step n e e' → nsteps erased_step n ([e], ()) ([e'], ()).
+  Proof.
+    intros.
+    SearchAbout nsteps.
+    cut (nsteps erased_step n ((fun e => ([e], ())) e) ((fun e => ([e], ())) e')). by simpl.
+    eapply nsteps_congruence; eauto.
+    intros. by apply pure_step_erased_step.
+  Qed.
+
+  Lemma steps_pure E ei' K e1' e2' n :
+    (nsteps pure_step n e1' e2') →
+    nclose specN ⊆ E →
+    initially_inv ei' ∗ currently_half (fill K e1') ={E}=∗ currently_half (fill K e2').
+  Proof.
+    iIntros (??) "[Hinv Hj]".
+    rewrite /initially_inv /initially_body.
+    iInv specN as ">Hinit" "Hclose".
+    iDestruct "Hinit" as (ef') "[Hown %]".
+    (** fill K e1' = ef' *)
+    rewrite /currently_half.
+    iDestruct (own_valid_2 with "Hown Hj") as "#eee".
+    rewrite -pair_op frac_op' Qp_half_half.
+    iDestruct "eee" as %[_ ->%agree_op_inv'%leibniz_equiv]%pair_valid.
+    (** update *)
+    (* bring together *)
+    iDestruct (equiv_entails_sym _ _ (own_op _ _ _) with "[Hj Hown]") as "HOwnOne".
+    iFrame.
+    (* actually update *)
+    rewrite -pair_op frac_op' Qp_half_half.
+    iMod (own_update _ _ (1%Qp, to_agree (fill K e2')) with "HOwnOne") as "HOwnOne".
+    rewrite agree_idemp.
+    { apply cmra_update_exclusive. done. }
+    rewrite -Qp_half_half -frac_op' -(agree_idemp (to_agree (fill K e2'))).
+    iDestruct "HOwnOne" as "[Hown1 Hown2]".
+    rewrite frac_op' Qp_half_half (agree_idemp (to_agree (fill K e2'))).
+    (** close invariant *)
+    iApply fupd_wand_r. iSplitL "Hclose Hown1". iApply ("Hclose" with "[Hown1]").
+    iNext. iExists (fill K e2'). iFrame.
+    iPureIntro. SearchAbout rtc. eapply rtc_transitive. apply H1.
+    apply (nsteps_rtc n). SearchAbout erased_step.
+    SearchAbout nsteps.
+    apply nsteps_pure_step_prim_step. by apply nsteps_pure_step_ctx.
+    iFrame "Hown2". done.
   Qed.
 
   Lemma step_fst E ei' K e1' e2' :
     AsVal e1' → AsVal e2' →
     nclose specN ⊆ E →
     initially_inv ei' ∗ currently_half (fill K (Fst (Pair e1' e2'))) ={E}=∗ currently_half (fill K e1').
-  Proof. intros [? <-] [? <-]. apply step_pure; econstructor; eauto. Qed.
+  Proof. intros [? <-] [? <-]. apply step_pure with (σ := tt); econstructor; eauto. Qed.
 
   Lemma step_snd E ei' K e1' e2' :
     AsVal e1' → AsVal e2' → nclose specN ⊆ E →
     initially_inv ei' ∗ currently_half (fill K (Snd (Pair e1' e2'))) ={E}=∗ currently_half (fill K e2').
-  Proof. intros [? <-] [? <-]; apply step_pure; econstructor; eauto. Qed.
+  Proof. intros [? <-] [? <-]. apply step_pure with (σ := tt); econstructor; eauto. Qed.
 
   Lemma step_lam E ei' K e1' e2' :
     AsVal e2' → nclose specN ⊆ E →
     initially_inv ei' ∗ currently_half (fill K (App (Lam e1') e2'))
     ={E}=∗ currently_half (fill K (e1'.[e2'/])).
-  Proof. intros [? <-]; apply step_pure; econstructor; eauto. Qed.
+  Proof. intros [? <-]; apply step_pure with (σ := tt); econstructor; eauto. Qed.
 
   Lemma step_Fold E ei' K e' :
     AsVal e' → nclose specN ⊆ E →
     initially_inv ei' ∗ currently_half (fill K (Unfold (Fold e'))) ={E}=∗ currently_half (fill K e').
-  Proof. intros [? <-]; apply step_pure; econstructor; eauto. Qed.
+  Proof. intros [? <-]; apply step_pure with (σ := tt); econstructor; eauto. Qed.
 
   Lemma step_case_inl E ei' K e0' e1' e2' :
     AsVal e0' → nclose specN ⊆ E →
     initially_inv ei' ∗ currently_half (fill K (Case (InjL e0') e1' e2'))
       ={E}=∗ currently_half (fill K (e1'.[e0'/])).
-  Proof. intros [? <-]; apply step_pure; econstructor; eauto. Qed.
+  Proof. intros [? <-]; apply step_pure with (σ := tt); econstructor; eauto. Qed.
 
   Lemma step_case_inr E ei' K e0' e1' e2' :
     AsVal e0' → nclose specN ⊆ E →
     initially_inv ei' ∗ currently_half (fill K (Case (InjR e0') e1' e2'))
       ={E}=∗ currently_half (fill K (e2'.[e0'/])).
-  Proof. intros [? <-]; apply step_pure; econstructor; eauto. Qed.
+  Proof. intros [? <-]; apply step_pure with (σ := tt); econstructor; eauto. Qed.
 End cfg.
