theories/refinements/static_gradual/compat_cast/tau_star.v
@@ -33,19 +33,18 @@ Section compat_cast_tau_star.
     iDestruct "Hfs" as "[% Hfs']"; iAssert (rel_cast_functions A fs) with "[Hfs']" as "Hfs". iSplit; done. iClear "Hfs'".
     wp_head. asimpl.
     fold (𝓕c pC1 fs). fold (𝓕c pC2 fs). do 2 rewrite 𝓕c_rewrite.
-    iApply (wp_bind (fill $ [stlc_mu.lang.AppRCtx _])).
+    iApply (wp_bind (ectx_language.fill $ [stlc_mu.lang.AppRCtx _])).
     iApply (wp_wand with "[-]").
     iMod (step_pure _ ei' K'
                     (Cast (# v') τ ⋆)
                     (Cast (Cast (# v') τ τG) τG ⋆) with "[Hv']") as "Hv'"; auto.
-    { eapply UpFactorization; auto. by eapply get_shape_is_ground. }
+    { eapply UpFactorization; auto. }
     rewrite -𝓕c_rewrite.
     iApply (IHpC1 ei' (CastCtx τG ⋆ :: K') with "[Hv']"); auto.
     iIntros (w) "blaa".  iDestruct "blaa" as (w') "[Hw' #Hww']".
     simpl.
     rewrite -𝓕c_rewrite.
     iApply (IHpC2 ei' K' with "[Hw']"); auto.
-    Unshelve. apply hack.
   Qed.
 
 End compat_cast_tau_star.
